Fail again...

theories/IPM.v
@@ -17,7 +17,6 @@ Set Typeclasses Depth 5.
 Section IRIS.
   Context {Σ: GRA.t}.
   Definition iProp := Σ -> Prop.
-  Definition Upd (P: iProp): iProp := fun r0 => forall ctx, URA.wf (r0 ⋅ ctx) -> exists r1, URA.wf (r1 ⋅ ctx) /\ P r1.
 
   Definition Sepconj (P Q: iProp): iProp :=
     fun r => exists a b, r = URA.add a b /\ P a /\ Q b
@@ -29,16 +28,19 @@ Section IRIS.
   Definition And (P Q: iProp): iProp := fun r => P r /\ Q r.
   Definition Or (P Q: iProp): iProp := fun r => P r \/ Q r.
   Definition Impl (P Q: iProp): iProp := fun r => URA.wf r -> P r -> Q r.
-  Definition Wand (P Q: iProp): iProp := fun r => forall rp, URA.wf (r ⋅ rp) -> P rp -> Upd Q (r ⋅ rp).
+  Definition Wand (P Q: iProp): iProp := fun r => forall rp, URA.wf (r ⋅ rp) -> P rp -> Q (r ⋅ rp).
 
-  Definition Entails (P Q: iProp): Prop := forall r (WF: URA.wf r), P r -> Upd Q r.
+  Definition Entails (P Q: iProp): Prop := forall r (WF: URA.wf r), P r -> Q r.
   Definition Impure (P: iProp): Prop := P ε.
 
-  Definition Emp `{M: GRA.t} : iProp := Pure True.
+  Definition Upd (P: iProp): iProp := fun r0 => forall ctx, URA.wf (r0 ⋅ ctx) -> exists r1, URA.wf (r1 ⋅ ctx) /\ P r1.
+
+  Definition Emp: iProp := eq ε.
+  Definition Persistently (P: iProp): iProp := fun _ => False.
 
   (* Trivial Ofe Structure *)
   Inductive uPred_equiv' (P Q : iProp) : Prop :=
-    { uPred_in_equiv : ∀ x, URA.wf x -> Upd P x <-> Upd Q x }.
+    { uPred_in_equiv : ∀ x, URA.wf x -> P x <-> Q x }.
 
   Local Instance uPred_equiv : Equiv iProp := uPred_equiv'.
   Definition uPred_dist' (n : nat) (P Q : iProp) : Prop := uPred_equiv' P Q.
@@ -52,20 +54,18 @@ Section IRIS.
     - i. split.
       + ii. ss.
       + ii. econs. i. symmetry. apply H. auto.
-      + ii. econs. i. transitivity (Upd y x0); [apply H|apply H0]; ss.
+      + ii. econs. i. transitivity (y x0); [apply H|apply H0]; ss.
     - i. ss.
   Qed.
   Canonical Structure uPredO : ofe := Ofe iProp uPred_ofe_mixin.
 
-  Program Definition uPred_compl : Compl uPredO := λ c x, forall n, Upd (c n) x.
+  Program Definition uPred_compl : Compl uPredO := λ c x, forall n, c n x.
 
   Global Program Instance uPred_cofe : Cofe uPredO := {| compl := uPred_compl |}.
   Next Obligation.
     econs. i. split.
-    - ii. exploit H0; et. i. des.
-      specialize (x1 n). exploit x1; et.
-    - ii. exists x. esplits; et.
-      ii. destruct (le_ge_dec n n0).
+    - ii. exploit H0; et.
+    - ii. destruct (le_ge_dec n n0).
       + apply c in l. apply l in H0; et.
       + apply c in g. apply g in H0; et.
   Qed.
@@ -73,125 +73,323 @@ Section IRIS.
 
   (* BI axioms *)
 
-  Lemma PreOrder_Entails: PreOrder Entails.
+  Global Program Instance PreOrder_Entails: PreOrder Entails.
+  Next Obligation.
   Proof.
-    econs.
-    { ii. exists r. splits; et. }
-    { ii. exploit (H r); et. i. des.
-      exploit (H0 r1); et. eapply URA.wf_mon; et. }
+    ii. ss.
+  Qed.
+  Next Obligation.
+  Proof.
+    ii. exploit (H r); et.
   Qed.
 
   Lemma equiv_Entails: ∀ P Q : iProp, P ≡ Q ↔ Entails P Q ∧ Entails Q P.
   Proof.
     econs.
-    { ii. split; red; i; eapply H; et.
-      { ii. exists r. splits; et. }
-      { ii. exists r. splits; et. }
-    }
+    { ii. split; red; i; eapply H; et. }
     { split. des. i. split; i.
-      { ii. exploit H2; et. i. des.
-        exploit (H r1); et. eapply URA.wf_mon; et. }
-      { ii. exploit H2; et. i. des.
-        exploit (H0 r1); et. eapply URA.wf_mon; et. }
+      { ii. exploit H0; et. }
+      { ii. exploit H; et. }
     }
   Qed.
 
   Lemma Pure_ne: ∀ n : nat, Proper (iff ==> dist n) Pure.
   Proof.
     econs. i. split.
-    { ii. exploit H1; et. i. des. esplits; et. eapply H. ss. }
-    { ii. exploit H1; et. i. des. esplits; et. eapply H3. ss. }
+    { ii. eapply H. ss. }
+    { ii. eapply H. ss. }
   Qed.
-
-  Goal ∀ P Q R : iProp, Entails P Q → Entails P R → Entails P (And Q R).
-  Proof.
-    i. unfold Entails, And in *. ii.
-    exploit (H r); et. i. des.
-    exploit (H0 r); et. i. des.
 
   Lemma And_ne: NonExpansive2 And.
   Proof.
     econs. i. split.
-    { ii. exploit H2; et. i. des. esplits ;et.
-      inv x3. split; auto.
-      { inv H.
+    { ii. inv H2. split.
+      { eapply H; et. }
+      { eapply H0; et. }
+    }
+    { ii. inv H2. split.
+      { eapply H; et. }
+      { eapply H0; et. }
+    }
+  Qed.
 
-        eapply H. red in H. red in H. red in H. red in H. eapply H.
+  Lemma Or_ne: NonExpansive2 Or.
+  Proof.
+    econs. i. split.
+    { ii. inv H2.
+      { left. eapply H; et. }
+      { right. eapply H0; et. }
+    }
+    { ii. inv H2.
+      { left. eapply H; et. }
+      { right. eapply H0; et. }
+    }
+  Qed.
 
-      inv H2.
+  Lemma Impl_ne: NonExpansive2 Impl.
+  Proof.
+    econs. i. split.
+    { ii. eapply H0; et. eapply H2; et. eapply H; et. }
+    { ii. eapply H0; et. eapply H2; et. eapply H; et. }
+  Qed.
 
-(* subgoal 4 (ID 40) is: *)
-(*  NonExpansive2 And *)
-(* subgoal 5 (ID 41) is: *)
-(*  NonExpansive2 Or *)
-(* subgoal 6 (ID 42) is: *)
-(*  NonExpansive2 Impl *)
-(* subgoal 7 (ID 43) is: *)
-(*  ∀ (A : Type) (n : nat), Proper (pointwise_relation A (dist n) ==> dist n) Univ *)
-(* subgoal 8 (ID 44) is: *)
-(*  ∀ (A : Type) (n : nat), Proper (pointwise_relation A (dist n) ==> dist n) Ex *)
-(* subgoal 9 (ID 45) is: *)
-(*  NonExpansive2 Sepconj *)
-(* subgoal 10 (ID 46) is: *)
-(*  NonExpansive2 Wand *)
-(* subgoal 11 (ID 47) is: *)
-(*  NonExpansive id *)
-(* subgoal 12 (ID 48) is: *)
-(*  ∀ (φ : Prop) (P : iProp), φ → Entails P (Pure φ) *)
-(* subgoal 13 (ID 49) is: *)
-(*  ∀ (φ : Prop) (P : iProp), (φ → Entails (Pure True) P) → Entails (Pure φ) P *)
-(* subgoal 14 (ID 50) is: *)
-(*  ∀ P Q : iProp, Entails (And P Q) P *)
-(* subgoal 15 (ID 51) is: *)
-(*  ∀ P Q : iProp, Entails (And P Q) Q *)
-(* subgoal 16 (ID 52) is: *)
-(*  ∀ P Q R : iProp, Entails P Q → Entails P R → Entails P (And Q R) *)
-(* subgoal 17 (ID 53) is: *)
-(*  ∀ P Q : iProp, Entails P (Or P Q) *)
-(* subgoal 18 (ID 54) is: *)
-(*  ∀ P Q : iProp, Entails Q (Or P Q) *)
-(* subgoal 19 (ID 55) is: *)
-(*  ∀ P Q R : iProp, Entails P R → Entails Q R → Entails (Or P Q) R *)
-(* subgoal 20 (ID 56) is: *)
-(*  ∀ P Q R : iProp, Entails (And P Q) R → Entails P (Impl Q R) *)
-(* subgoal 21 (ID 57) is: *)
-(*  ∀ P Q R : iProp, Entails P (Impl Q R) → Entails (And P Q) R *)
-(* subgoal 22 (ID 58) is: *)
-(*  ∀ (A : Type) (P : iProp) (Ψ : A → iProp), (∀ a : A, Entails P (Ψ a)) → Entails P (Univ (λ a : A, Ψ a)) *)
-(* subgoal 23 (ID 59) is: *)
-(*  ∀ (A : Type) (Ψ : A → iProp) (a : A), Entails (Univ (λ a0 : A, Ψ a0)) (Ψ a) *)
-(* subgoal 24 (ID 60) is: *)
-(*  ∀ (A : Type) (Ψ : A → iProp) (a : A), Entails (Ψ a) (Ex (λ a0 : A, Ψ a0)) *)
-(* subgoal 25 (ID 61) is: *)
-(*  ∀ (A : Type) (Φ : A → iProp) (Q : iProp), (∀ a : A, Entails (Φ a) Q) → Entails (Ex (λ a : A, Φ a)) Q *)
-(* subgoal 26 (ID 62) is: *)
-(*  ∀ P P' Q Q' : iProp, Entails P Q → Entails P' Q' → Entails (Sepconj P P') (Sepconj Q Q') *)
-(* subgoal 27 (ID 63) is: *)
-(*  ∀ P : iProp, Entails P (Sepconj Emp P) *)
-(* subgoal 28 (ID 64) is: *)
-(*  ∀ P : iProp, Entails (Sepconj Emp P) P *)
-(* subgoal 29 (ID 65) is: *)
-(*  ∀ P Q : iProp, Entails (Sepconj P Q) (Sepconj Q P) *)
-(* subgoal 30 (ID 66) is: *)
-(*  ∀ P Q R : iProp, Entails (Sepconj (Sepconj P Q) R) (Sepconj P (Sepconj Q R)) *)
-(* subgoal 31 (ID 67) is: *)
-(*  ∀ P Q R : iProp, Entails (Sepconj P Q) R → Entails P (Wand Q R) *)
-(* subgoal 32 (ID 68) is: *)
-(*  ∀ P Q R : iProp, Entails P (Wand Q R) → Entails (Sepconj P Q) R *)
-(* subgoal 33 (ID 69) is: *)
-(*  ∀ P Q : iProp, Entails P Q → Entails (id P) (id Q) *)
-(* subgoal 34 (ID 70) is: *)
-(*  ∀ P : iProp, Entails (id P) (id (id P)) *)
-(* subgoal 35 (ID 71) is: *)
-(*  Entails Emp (id Emp) *)
-(* subgoal 36 (ID 72) is: *)
-(*  ∀ (A : Type) (Ψ : A → iProp), Entails (Univ (λ a : A, id (Ψ a))) (id (Univ (λ a : A, Ψ a))) *)
-(* subgoal 37 (ID 73) is: *)
-(*  ∀ (A : Type) (Ψ : A → iProp), Entails (id (Ex (λ a : A, Ψ a))) (Ex (λ a : A, id (Ψ a))) *)
-(* subgoal 38 (ID 74) is: *)
-(*  ∀ P Q : iProp, Entails (Sepconj (id P) Q) (id P) *)
-(* subgoal 39 (ID 75) is: *)
-(*  ∀ P Q : iProp, Entails (And (id P) Q) (Sepconj P Q) *)
+  Lemma Sepconj_ne: NonExpansive2 Sepconj.
+  Proof.
+    econs. i. split.
+    { ii. inv H2. des. subst. eexists. esplits; eauto.
+      { eapply H; et. eapply URA.wf_mon; et. }
+      { eapply H0; et. eapply URA.wf_mon; et. rewrite URA.add_comm. et. }
+    }
+    { ii. inv H2. des. subst. eexists. esplits; eauto.
+      { eapply H; et. eapply URA.wf_mon; et. }
+      { eapply H0; et. eapply URA.wf_mon; et. rewrite URA.add_comm. et. }
+    }
+  Qed.
+
+  Lemma Wand_ne: NonExpansive2 Wand.
+  Proof.
+    econs. i. split.
+    { ii. exploit H2; et.
+      { eapply H; et. eapply URA.wf_mon; et. rewrite URA.add_comm. et. }
+      { i. eapply H0; et. }
+    }
+    { ii. exploit H2; et.
+      { eapply H; et. eapply URA.wf_mon; et. rewrite URA.add_comm. et. }
+      { i. eapply H0; et. }
+    }
+  Qed.
+
+  Lemma Persistently_ne: NonExpansive Persistently.
+  Proof.
+    ii. ss.
+  Qed.
+
+  Lemma Univ_ne: ∀ (A : Type) (n : nat), Proper (pointwise_relation A (dist n) ==> dist n) Univ.
+  Proof.
+    econs. i. split.
+    { ii. exploit H; et. i. eapply x2; et. }
+    { ii. exploit H; et. i. eapply x2; et. }
+  Qed.
+
+  Lemma Ex_ne: ∀ (A : Type) (n : nat), Proper (pointwise_relation A (dist n) ==> dist n) Ex.
+  Proof.
+    econs. i. split.
+    { ii. inv H1. exploit H; et. i. eexists. eapply x2; et. }
+    { ii. inv H1. exploit H; et. i. eexists. eapply x2; et. }
+  Qed.
+
+  Lemma Pure_intro: ∀ (φ : Prop) (P : iProp), φ → Entails P (Pure φ).
+  Proof.
+    ii. ss.
+  Qed.
+
+  Lemma Pure_elim: ∀ (φ : Prop) (P : iProp), (φ → Entails (Pure True) P) → Entails (Pure φ) P.
+  Proof.
+    ii. eapply H in H0. eapply H0; ss.
+  Qed.
+
+  Lemma And_elim_l: ∀ P Q : iProp, Entails (And P Q) P.
+  Proof.
+    ii. eapply H.
+  Qed.
+
+  Lemma And_elim_r: ∀ P Q : iProp, Entails (And P Q) Q.
+  Proof.
+    ii. eapply H.
+  Qed.
+
+  Lemma And_intro: ∀ P Q R : iProp, Entails P Q → Entails P R → Entails P (And Q R).
+  Proof.
+    ii. split; et.
+  Qed.
+
+  Lemma Or_intro_l: ∀ P Q : iProp, Entails P (Or P Q).
+  Proof.
+    ii. left. ss.
+  Qed.
+
+  Lemma Or_intro_r: ∀ P Q : iProp, Entails Q (Or P Q).
+  Proof.
+    ii. right. ss.
+  Qed.
+
+  Lemma Or_elim: ∀ P Q R : iProp, Entails P R → Entails Q R → Entails (Or P Q) R.
+  Proof.
+    ii. inv H1.
+    { eapply H; ss. }
+    { eapply H0; ss. }
+  Qed.
+
+  Lemma Impl_intro_r: ∀ P Q R : iProp, Entails (And P Q) R → Entails P (Impl Q R).
+  Proof.
+    ii. eapply H; et. split; ss.
+  Qed.
+
+  Lemma Impl_elim_l: ∀ P Q R : iProp, Entails P (Impl Q R) → Entails (And P Q) R.
+  Proof.
+    ii. inv H0. eapply H; et.
+  Qed.
+
+  Lemma Univ_intro: ∀ (A : Type) (P : iProp) (Ψ : A → iProp), (∀ a : A, Entails P (Ψ a)) → Entails P (Univ (λ a : A, Ψ a)).
+  Proof.
+    ii. eapply H; et.
+  Qed.
+
+  Lemma Univ_elim: ∀ (A : Type) (Ψ : A → iProp) (a : A), Entails (Univ (λ a0 : A, Ψ a0)) (Ψ a).
+  Proof.
+    ii. eapply H; et.
+  Qed.
+
+  Lemma Ex_intro: ∀ (A : Type) (Ψ : A → iProp) (a : A), Entails (Ψ a) (Ex (λ a0 : A, Ψ a0)).
+  Proof.
+    ii. eexists. eauto.
+  Qed.
+
+  Lemma Ex_elim: ∀ (A : Type) (Φ : A → iProp) (Q : iProp), (∀ a : A, Entails (Φ a) Q) → Entails (Ex (λ a : A, Φ a)) Q.
+  Proof.
+    ii. inv H0. eapply H; et.
+  Qed.
+
+  Lemma Sepconj_mono: ∀ P P' Q Q' : iProp, Entails P Q → Entails P' Q' → Entails (Sepconj P P') (Sepconj Q Q').
+  Proof.
+    ii. unfold Sepconj in *. des; subst. esplits; et.
+    { eapply H; et. eapply URA.wf_mon; et. }
+    { eapply H0; et. eapply URA.wf_mon; et. rewrite URA.add_comm. et. }
+  Qed.
+
+  Lemma Emp_Sepconj_l: ∀ P : iProp, Entails P (Sepconj Emp P).
+  Proof.
+    ii. exists ε, r. splits; ss. rewrite URA.unit_idl. et.
+  Qed.
+
+  Lemma Emp_Sepconj_r: ∀ P : iProp, Entails (Sepconj Emp P) P.
+  Proof.
+    ii. inv H. des; subst. inv H1. rewrite URA.unit_idl. et.
+  Qed.
+
+  Lemma Sepconj_comm: ∀ P Q : iProp, Entails (Sepconj P Q) (Sepconj Q P).
+  Proof.
+    ii. unfold Sepconj in *. des. subst. exists b, a. splits; et. apply URA.add_comm.
+  Qed.
+
+  Lemma Sepconj_assoc: ∀ P Q R : iProp, Entails (Sepconj (Sepconj P Q) R) (Sepconj P (Sepconj Q R)).
+  Proof.
+    ii. unfold Sepconj in *. des; subst. esplits; [|apply H2| |apply H3|apply H1]; ss.
+    rewrite URA.add_assoc. ss.
+  Qed.
+
+  Lemma Wand_intro_r: ∀ P Q R : iProp, Entails (Sepconj P Q) R → Entails P (Wand Q R).
+  Proof.
+    ii. eapply H; et. exists r, rp. splits; et.
+  Qed.
+
+  Lemma Wand_elim_l: ∀ P Q R : iProp, Entails P (Wand Q R) → Entails (Sepconj P Q) R.
+  Proof.
+    ii. unfold Sepconj in *. des; subst. eapply H; et. eapply URA.wf_mon; et.
+  Qed.
+
+  Lemma Persistently_mono: ∀ P Q : iProp, Entails P Q → Entails (Persistently P) (Persistently Q).
+  Proof.
+    ii. ss.
+  Qed.
+
+  Lemma Persistently_idemp: ∀ P : iProp, Entails (Persistently P) (Persistently (Persistently P)).
+  Proof.
+    ii. ss.
+  Qed.
+
+  Lemma Persistently_Univ: ∀ (A : Type) (Ψ : A → iProp), Entails (Univ (λ a : A, id (Ψ a))) ((Univ (λ a : A, Ψ a))).
+  Proof.
+    ii. ss.
+  Qed.
+
+  Lemma Persistently_Ex: ∀ (A : Type) (Ψ : A → iProp), Entails (id (Ex (λ a : A, Ψ a))) (Ex (λ a : A, id (Ψ a))).
+  Proof.
+    ii. ss.
+  Qed.
+
+  Lemma Persistently_Sepconj: ∀ P Q : iProp, Entails (Sepconj (Persistently P) Q) (Persistently P).
+  Proof.
+    ii. unfold Sepconj in *. des; subst. ss.
+  Qed.
+
+  Lemma Persistently_And: ∀ P Q : iProp, Entails (And (Persistently P) Q) (Sepconj P Q).
+  Proof.
+    ii. inv H. ss.
+  Qed.
+
+  Lemma uPred_bi_mixin:
+    BiMixin
+      Entails Emp Pure And Or Impl
+      (@Univ) (@Ex) Sepconj Wand
+      Persistently.
+  Proof.
+    econs.
+    - exact PreOrder_Entails.
+    - exact equiv_Entails.
+    - exact Pure_ne.
+    - exact And_ne.
+    - exact Or_ne.
+    - exact Impl_ne.
+    - exact Univ_ne.
+    - exact Ex_ne.
+    - exact Sepconj_ne.
+    - exact Wand_ne.
+    - exact Persistently_ne.
+    - exact Pure_intro.
+    - exact Pure_elim.
+    - exact And_elim_l.
+    - exact And_elim_r.
+    - exact And_intro.
+    - exact Or_intro_l.
+    - exact Or_intro_r.
+    - exact Or_elim.
+    - exact Impl_intro_r.
+    - exact Impl_elim_l.
+    - exact Univ_intro.
+    - exact Univ_elim.
+    - exact Ex_intro.
+    - exact Ex_elim.
+    - exact Sepconj_mono.
+    - exact Emp_Sepconj_l.
+    - exact Emp_Sepconj_r.
+    - exact Sepconj_comm.
+    - exact Sepconj_assoc.
+    - exact Wand_intro_r.
+    - exact Wand_elim_l.
+    - exact Persistently_mono.
+    - exact Persistently_idemp.
+    - ii. ss.
+
+  : ∀ P : iProp, Entails (Persistently P) (Persistently (Persistently P)).
+  Proof.
+    ii. ss.
+  Qed.
+
+  Lemma Persistently_Univ: ∀ (A : Type) (Ψ : A → iProp), Entails (Univ (λ a : A, id (Ψ a))) ((Univ (λ a : A, Ψ a))).
+  Proof.
+    ii. ss.
+  Qed.
+
+  Lemma Persistently_Ex: ∀ (A : Type) (Ψ : A → iProp), Entails (id (Ex (λ a : A, Ψ a))) (Ex (λ a : A, id (Ψ a))).
+  Proof.
+    ii. ss.
+  Qed.
+
+  Lemma Persistently_Sepconj: ∀ P Q : iProp, Entails (Sepconj (Persistently P) Q) (Persistently P).
+  Proof.
+    ii. unfold Sepconj in *. des; subst. ss.
+  Qed.
+
+  Lemma Persistently_And: ∀ P Q : iProp, Entails (And (Persistently P) Q) (Sepconj P Q).
+  Proof.
+    ii. inv H. ss.
+  Qed.
+
+
+
+  Admitted.
+
 
 (*   NonExpansive id *)
 
